use zave invariant to prove live node exists

systems/chord-props/RingCorrect.v
@@ -1,29 +1,25 @@
 Require Import List.
+Require Import Omega.
+Require Import StructTact.StructTactics.
 
 Require Import Chord.Chord.
 Require Import Chord.SystemReachable.
-
-Definition at_least_one_ring (gst : global_state) : Prop :=
-  exists h, ring_member gst h.
-
-Definition at_most_one_ring (gst : global_state) : Prop :=
-  forall x y,
-    ring_member gst x ->
-    ring_member gst y ->
-    reachable gst x y.
-
-Definition connected_appendages (gst : global_state) : Prop :=
-  forall a, live_node gst a ->
-       exists r, ring_member gst r /\ reachable gst a r.
 
 Definition sufficient_principals (gst : global_state) : Prop :=
   exists ps,
     principals gst ps /\
     length ps > SUCC_LIST_LEN.
 
-Definition state_invariant (gst : global_state) : Prop :=
+Definition zave_invariant (gst : global_state) : Prop :=
   sufficient_principals gst /\
   live_node_in_succ_lists gst.
+
+Theorem zave_invariant_holds :
+  forall gst,
+    reachable_st gst ->
+    zave_invariant gst.
+Proof.
+Admitted.
 
 Lemma first_succ_and_others_distinct :
   forall gst h st s1 s2 xs ys,
